Uppaal_Networks/AbsInt/Word.thy
@@ -1,5 +1,5 @@
 theory Word
-  imports AbsInt PowerBool
+  imports AbsInt PowerBool Toption
 begin
 
 section \<open>Abstraction of Machine Words\<close>
@@ -11,6 +11,7 @@ locale AbsWord =
 fixes \<gamma>_word :: "('a::absword) \<Rightarrow> int set"
   and contains :: "'a \<Rightarrow> int \<Rightarrow> bool"
   and make :: "int \<Rightarrow> 'a"
+  and concretize :: "'a \<Rightarrow> int set toption" \<comment> \<open>Finite overapproximation of \<gamma>_word if existing\<close>
   and aplus :: "'a \<Rightarrow> 'a \<Rightarrow> 'a"
   and lt :: "'a \<Rightarrow> 'a \<Rightarrow> power_bool"
   and le :: "'a \<Rightarrow> 'a \<Rightarrow> power_bool"
@@ -19,6 +20,8 @@ assumes mono_gamma: "a \<le> b \<Longrightarrow> \<gamma>_word a \<le> \<gamma>_
   and gamma_Top[simp]: "\<gamma>_word \<top> = \<top>"
   and contains_correct: "contains a x \<longleftrightarrow> x \<in> \<gamma>_word a"
   and make_correct: "v \<in> \<gamma>_word (make v)"
+  and concretize_correct: "concretize a = Minor vs \<Longrightarrow> \<gamma>_word a \<subseteq> vs"
+  and concretize_finite: "concretize a = Minor vs \<Longrightarrow> finite vs"
   and plus_correct: "x \<in> \<gamma>_word a \<Longrightarrow> y \<in> \<gamma>_word b \<Longrightarrow> (x + y) \<in> \<gamma>_word (aplus a b)"
   and lt_correct: "lt a b = (     if \<forall>x y. x \<in> \<gamma>_word a \<longrightarrow> y \<in> \<gamma>_word b \<longrightarrow> x < y then BTrue
                              else if \<exists>x y. x \<in> \<gamma>_word a \<longrightarrow> y \<in> \<gamma>_word b \<longrightarrow> x < y then BBoth
